code/experimental/chacha20/Hacl.Impl.Chacha20.Core32.fst
@@ -4,8 +4,10 @@ module ST = FStar.HyperStack.ST
 open FStar.HyperStack
 open FStar.HyperStack.All
 open Lib.IntTypes
+open Lib.Sequence
 open Lib.Buffer
 open Lib.ByteBuffer
+module Spec = Spec.Chacha20
 
 let state = lbuffer uint32 16ul
 let index = (i:size_t{size_v i < 16})
@@ -13,20 +15,32 @@ let index = (i:size_t{size_v i < 16})
 inline_for_extraction
 val create_state: unit -> StackInline state
 		  (requires (fun h -> True))
-   		  (ensures (fun h0 r h1 -> live h1 r /\ stack_allocated r h0 h1 (Seq.create 16 (u32 0))))
+   		  (ensures (fun h0 r h1 -> live h1 r /\ 
+					as_seq h1 r == Seq.create 16 (u32 0) /\
+					stack_allocated r h0 h1 (Seq.create 16 (u32 0))))
 let create_state () = create (size 16) (u32 0) 
 
 inline_for_extraction
 val load_state: st:state -> b:lbuffer uint8 64ul -> ST unit
 		  (requires (fun h -> live h st /\ live h b))
-   		  (ensures (fun h0 _ h1 -> modifies (loc st) h0 h1))
+   		  (ensures (fun h0 _ h1 -> modifies (loc st) h0 h1 /\
+			   as_seq h1 st == Lib.ByteSequence.uints_from_bytes_le (as_seq h0 b)))
 let load_state st b =
     uints_from_bytes_le st b
 
 inline_for_extraction
+val store_state: b:lbuffer uint8 64ul -> st:state -> ST unit
+		  (requires (fun h -> live h st /\ live h b))
+   		  (ensures (fun h0 _ h1 -> modifies (loc b) h0 h1 /\
+		    as_seq h1 b == Lib.ByteSequence.uints_to_bytes_le (as_seq h0 st)))
+let store_state st b =
+    uints_to_bytes_le 16ul st b
+
+inline_for_extraction
 val set_counter: st:state -> c:size_t -> ST unit
 		  (requires (fun h -> live h st))
-   		  (ensures (fun h0 _ h1 -> modifies (loc st) h0 h1))
+   		  (ensures (fun h0 _ h1 -> modifies (loc st) h0 h1 /\
+			   as_seq h1 st == Seq.upd (as_seq h0 st) 12 (size_to_uint32 c)))
 let set_counter st c =
     st.(size 12) <- size_to_uint32 c
 
@@ -41,41 +55,42 @@ let incr_counter st =
 inline_for_extraction
 val copy_state: st:state -> ost:state -> ST unit
 		  (requires (fun h -> live h st /\ live h ost /\ disjoint st ost))
-   		  (ensures (fun h0 _ h1 -> modifies (loc st) h0 h1))
-let copy_state st ost =
-    copy st ost
+   		  (ensures (fun h0 _ h1 -> 
+		    modifies (loc st) h0 h1 /\
+		    as_seq h1 st == as_seq h0 ost))
+let copy_state st ost = copy #MUT #uint32 #(size 16) st ost
 
 
 inline_for_extraction
 val sum_state: st:state -> ost:state -> ST unit
-		  (requires (fun h -> live h st /\ live h ost))
-   		  (ensures (fun h0 _ h1 -> modifies (loc st) h0 h1))
-let sum_state st ost =
-    let h0 = ST.get() in
-    loop_nospec #h0 (size 16) st 
-      (fun i -> let si = st.(i) in
-	     let osi = ost.(i) in
-	     st.(i) <- si +. osi)
-
-
+		  (requires (fun h -> live h st /\ live h ost /\ eq_or_disjoint st ost))
+   		  (ensures (fun h0 _ h1 -> 
+		    modifies (loc st) h0 h1 /\
+		    as_seq h1 st == Lib.Sequence.map2 ( +. ) (as_seq h0 st) (as_seq h0 ost)))
+let sum_state st ost =  map2T #MUT #uint32 #uint32 #uint32 (size 16) st ( +. ) st ost
+      
 
 inline_for_extraction
 val xor_block: o:lbuffer uint8 64ul -> st:state -> b:lbuffer uint8 64ul -> ST unit
 		  (requires (fun h -> live h o /\ live h st /\ live h b))
-   		  (ensures (fun h0 _ h1 -> modifies (loc o) h0 h1))
+   		  (ensures (fun h0 _ h1 -> modifies (loc o) h0 h1 /\
+					as_seq h1 o == Spec.xor_block (as_seq h0 st) (as_seq h0 b)))
 let xor_block o st b =
+    push_frame();
+    let bl = create_state() in
+    load_state bl b;
     let h0 = ST.get () in
-    loop_nospec #h0 (size 16) o 
-      (fun i -> 
-	let u = uint_from_bytes_le (sub b (i *. size 4) (size 4)) in
-        uint_to_bytes_le (sub o (i *. size 4) (size 4)) (u ^. st.(i)))
+    map2T (size 16) bl ( ^. ) bl st;
+    store_state o bl;
+    pop_frame()
     
-    
+
 
 inline_for_extraction
 val line: st:state -> a:index -> b:index -> d:index -> r:rotval U32 -> ST unit
-		  (requires (fun h -> live h st))
-		  (ensures (fun h0 _ h1 -> modifies (loc st) h0 h1))
+		  (requires (fun h -> live h st /\ v a <> v d))
+		  (ensures (fun h0 _ h1 -> modifies (loc st) h0 h1 /\
+		    as_seq h1 st == Spec.line (v a) (v b) (v d) r (as_seq h0 st)))
 let line st a b d r = 
   let sta = st.(a) in
   let stb = st.(b) in
@@ -86,11 +101,11 @@ let line st a b d r =
   st.(a) <- sta;
   st.(d) <- std
 
-
 inline_for_extraction
 val quarter_round: st:state -> a:index -> b:index -> c:index -> d:index -> ST unit
-		  (requires (fun h -> live h st))
-		  (ensures (fun h0 _ h1 -> modifies (loc st) h0 h1))
+		  (requires (fun h -> live h st /\ v a <> v d /\ v c <> v b))
+		  (ensures (fun h0 _ h1 -> modifies (loc st) h0 h1 /\
+			   as_seq h1 st == Spec.quarter_round (v a) (v b) (v c) (v d) (as_seq h0 st)))
 [@ CInline ]
 let quarter_round st a b c d = 
     line st a b d (size 16);
@@ -101,7 +116,8 @@ let quarter_round st a b c d =
 [@ CInline]
 val double_round: st:state -> ST unit
 		  (requires (fun h -> live h st))
-		  (ensures (fun h0 _ h1 -> modifies (loc st) h0 h1))
+		  (ensures (fun h0 _ h1 -> modifies (loc st) h0 h1 /\
+		    as_seq h1 st == Spec.double_round (as_seq h0 st)))
 [@ CInline]
 let double_round st = 
   quarter_round st (size 0) (size 4) (size 8) (size 12);
