lib/Lib.Buffer.fsti
@@ -811,16 +811,29 @@ val fill:
   -> clen:size_t
   -> o:lbuffer a clen
   -> spec:(mem -> GTot(i:size_nat{i < v clen} -> a))
-  -> impl:(i:size_t{v i < v clen} -> Stack unit
-          (requires fun h -> modifies1 o h0 h)
-          (ensures  fun h _ h' ->
-            modifies1 o h h' /\
-            as_seq h' o == Seq.upd (as_seq h o) (v i) (spec h0 (v i))))
+  -> impl:(i:size_t{v i < v clen} -> Stack a
+          (requires fun h -> modifies1 (gsub o 0ul i) h0 h)
+          (ensures  fun h r h' -> h == h' /\ 
+			       r == spec h0 (v i ))) 
   -> Stack unit
     (requires fun h -> h == h0 /\ live h0 o)
     (ensures  fun h _ h' ->
       modifies1 o h h' /\
       as_seq h' o == Seq.createi #a (v clen) (spec h0))
+
+inline_for_extraction noextract
+let eq_or_disjoint
+    (#t1:buftype)
+    (#t2:buftype)
+    (#a1:Type)
+    (#a2:Type)
+    (#clen1:size_t)
+    (#clen2:size_t)
+    (b1:lbuffer_t t1 a1 clen1)
+    (b2:lbuffer_t t2 a2 clen2) = 
+    disjoint b1 b2 \/
+    (t1 == t2 /\ a1 == a2 /\ clen1 == clen2 /\ b1 == b2)
+
 
 (** Map a total function onto a buffer *)
 inline_for_extraction
@@ -833,10 +846,28 @@ val mapT:
   -> f:(a -> Tot b)
   -> i:lbuffer_t t a clen ->
   Stack unit
-    (requires fun h0 -> live h0 o /\ live h0 i /\ disjoint o i)
+    (requires fun h0 -> live h0 o /\ live h0 i /\ eq_or_disjoint o i)
     (ensures  fun h0 _ h1 ->
       modifies1 o h0 h1 /\
       as_seq h1 o == Seq.map f (as_seq h0 i))
+
+inline_for_extraction
+val map2T:
+    #t:buftype
+  -> #a1:Type
+  -> #a2:Type
+  -> #b:Type
+  -> clen:size_t
+  -> o:lbuffer b clen
+  -> f:(a1 -> a2 -> Tot b)
+  -> i1:lbuffer_t t a1 clen 
+  -> i2:lbuffer_t t a2 clen ->
+  Stack unit
+    (requires fun h0 -> live h0 o /\ live h0 i1 /\ live h0 i2 /\ 
+		     eq_or_disjoint o i1 /\ eq_or_disjoint o i2)
+    (ensures  fun h0 _ h1 ->
+      modifies1 o h0 h1 /\
+      as_seq h1 o == Seq.map2 f (as_seq h0 i1) (as_seq h0 i2))
 
 (** Map a total function (depending on the index) onto a buffer *)
 inline_for_extraction
@@ -849,7 +880,7 @@ val mapiT:
   -> f:(i:size_t{v i < v clen} -> x:a -> r:b)
   -> i:lbuffer_t t a clen ->
   Stack unit
-    (requires fun h0 -> live h0 o /\ live h0 i /\ disjoint o i)
+    (requires fun h0 -> live h0 o /\ live h0 i /\ eq_or_disjoint o i)
     (ensures  fun h0 _ h1 ->
       modifies1 o h0 h1 /\
       as_seq h1 o == Seq.mapi (fun i -> f (size i)) (as_seq h0 i))
@@ -864,11 +895,47 @@ val mapi:
   -> o:lbuffer b clen
   -> spec_f:(mem -> GTot (i:size_nat{i < v clen} -> a -> b))
   -> f:(i:size_t{v i < v clen} -> x:a -> Stack b
-      (requires fun _ -> True)
-      (ensures  fun h y h1 -> y == spec_f h0 (v i) x /\ modifies0 h h1))
+      (requires fun h -> modifies1 o h0 h)
+      (ensures  fun h y h1 -> h == h1 /\ y == spec_f h0 (v i) x))
   -> i:lbuffer a clen ->
   Stack unit
-    (requires fun h -> h == h0 /\ live h0 o /\ live h0 i /\ disjoint o i)
+    (requires fun h -> h == h0 /\ live h0 o /\ live h0 i /\ eq_or_disjoint o i)
     (ensures  fun h _ h1 ->
       modifies1 o h h1 /\
       as_seq h1 o == Seq.mapi (spec_f h0) (as_seq h i))
+
+#set-options "--z3rlimit 50"
+(*
+inline_for_extraction noextract
+val map_blocks:
+    #t:buftype
+  -> #a:Type0
+  -> #len:size_t
+  -> h0: mem
+  -> blocksize:size_t{v blocksize > 0}
+  -> inp:lbuffer_t t a len 
+  -> output:lbuffer a len{eq_or_disjoint inp output}
+  -> spec_f:(mem -> GTot (i:nat{i < v len / v blocksize} -> Seq.lseq a (v blocksize) -> Seq.lseq a (v blocksize)))
+  -> spec_l:(mem -> GTot (i:nat{i <= v len / v blocksize} -> llen:size_nat{llen < v blocksize} -> Seq.lseq a llen -> Seq.lseq a llen))
+  -> impl_f:(i:size_t{v i < v len / v blocksize} -> Stack unit
+      (requires fun h1 ->	modifies1 (gsub output 0ul (i *. blocksize)) h0 h1)
+      (ensures  fun h1 _ h2 -> 
+	v i * v blocksize + v blocksize <= v len /\
+       (let block = gsub output (i *. blocksize) blocksize in
+	modifies1 block h1 h2 /\
+	as_seq h2 block == spec_f h0 (v i) (as_seq h1 block))))
+  -> impl_l:(i:size_t{v i == v len / v blocksize} -> Stack unit
+      (requires fun h1 ->	
+	modifies1 (gsub output 0ul (i *. blocksize)) h0 h1)
+      (ensures  fun h1 _ h2 -> 
+	v i * v blocksize + (v len % v blocksize) == v len /\
+       (let block = gsub output (i *. blocksize) (len %. blocksize) in
+	modifies1 block h1 h2 /\
+	as_seq h2 block == spec_l h0 (v i) (v len % v blocksize) (as_seq h1 block))))
+  -> Stack unit
+    (requires fun h -> h0 == h /\ live h output)
+    (ensures  fun _ _ h1 -> modifies1 output h0 h1 /\
+	as_seq h1 output == Seq.map_blocks (v blocksize) (as_seq h0 inp) (spec_f h0) (spec_l h0))
+	  
+*)
+  
